tests/lean/run/smt_destruct.lean
@@ -6,3 +6,43 @@ by using_smt $ do
    a_1 ← tactic.get_local `a_1,
    destruct a_1,
    repeat close
+
+example (p q : Prop) : p ∨ q → p ∨ ¬q → ¬p ∨ q → ¬p ∨ ¬q → false :=
+begin [smt]
+   assert h : p ∨ q,
+   destruct h
+end
+
+example (p q : Prop) : p ∨ q → p ∨ ¬q → ¬p ∨ q → ¬p ∨ ¬q → false :=
+begin [smt]
+   destruct a_1 -- bad style, it relies on automatically generated names
+end
+
+example (p q : Prop) : p ∨ q → p ∨ ¬q → ¬p ∨ q → ¬p ∨ ¬q → false :=
+begin [smt] -- the default configuration is classical
+   by_cases p
+end
+
+example (p q : Prop) [decidable p] : p ∨ q → p ∨ ¬q → ¬p ∨ q → ¬p ∨ ¬q → false :=
+begin [smt] with default_smt_config^.set_classical ff,
+   by_cases p -- will fail if p is not decidable
+end
+
+example (p q : Prop) : p ∨ q → p ∨ ¬q → ¬p ∨ q → p ∧ q :=
+begin [smt] -- the default configuration is classical
+  by_contradiction,
+  trace_state,
+  by_cases p,
+end
+
+example (p q : Prop) [decidable p] : p ∨ q → p ∨ ¬q → ¬p ∨ q → p ∧ q :=
+begin [smt] with default_smt_config^.set_classical ff,
+   by_cases p -- will fail if p is not decidable
+end
+
+example (p q : Prop) [decidable p] [decidable q] : p ∨ q → p ∨ ¬q → ¬p ∨ q → p ∧ q :=
+begin [smt] with default_smt_config^.set_classical ff,
+   by_contradiction, -- will fail if p or q is not decidable
+   trace_state,
+   by_cases p -- will fail if p is not decidable
+end
